max subseq recurrence wip

dp/problems.dfy
@@ -7,28 +7,41 @@ predicate sumOfEmptySubseq(subSeq: seq<int>, sum: int)
     |subSeq| == 0 ==> sum == 0
 }
 
-predicate sumOfSingletonSeq(sequences: seq<int>, sum: int) 
+// Post-condition(s):
+predicate maxSubseqSum(sequence: seq<int>, sum: int)
 {
-    |sequences| == 1 ==> sum == 0
+    // Do we need a total ordering such as this? Or less strict?
+    forall i, j :: 0 <= i < j <= |sequence| ==> sum > Prop.seqSum(sequence[i..j])
 }
 
 // (TODO) Recurrence of contiguous subsequence of maxium sum:
-function recMaxContiguousSubseq(s: seq<int>, i: int): int
-requires 0 <= i < |s|
+// (TODO) Can probably do away with index i?
+function recMaxContiguousSubseq(sequence: seq<int>, subSeq: seq<int>, i: int): int
+decreases |sequence| - i
+requires 0 <= i < |sequence|
 {
-    if i-1 < 0 
+    // Base case.
+    if i == |sequence| then sequence[i-1] else
+    if |sequence| == |subSeq| 
+        then recMaxContiguousSubseq(sequence[i+1..], sequence[i+1..i+2], 0)
+    else if Prop.seqSum(subSeq) > recMaxContiguousSubseq(sequence, sequence[..i+1], i+1)
+        then Prop.seqSum(subSeq) else recMaxContiguousSubseq(sequence, sequence[..i+1], i+1)
+
+    /*
+    if i == 0 
         then 0
     else
     if s[i] > s[i] + recMaxContiguousSubseq(s, i-1)
         then s[i]
     else s[i] + recMaxContiguousSubseq(s, i-1)
+    */
 }
 
 method maxContiguousSubseq(a: seq<int>) returns (subSeq: seq<int>, sum: int)
 ensures Prop.shorterThan(subSeq, a)
 ensures Prop.subsetOf(subSeq, a)
 ensures Prop.increasing(subSeq) // or strictly increasing?
+ensures maxSubseqSum(a, sum)
 ensures sumOfEmptySubseq(subSeq, sum)
-ensures sumOfSingletonSeq(a, sum)
 {
 }
